---
title: "Recommended Exercise 7 in Statistical Linear Models, Spring 2021"
author: "alexaoh"
date: "`r format(Sys.time(), '%d %B, %Y')`"
output: pdf_document
---

```{r setup, include=FALSE}
knitr::opts_chunk$set(echo = TRUE, eval = TRUE, comment = "#>", message = F, warning = F, cache = T)
```

\textcolor{red}{GÃ¥ skikkelig gjennom LF senere!}

# Problem 1 \hspace{3mm} Inference about a new observation in multiple linear regression

## a)

Since $\hat{\boldsymbol{\beta}} = (X^TX)^{-1}X^T\boldsymbol{Y}$, we know that $\hat{\boldsymbol{\beta}} \sim N(\boldsymbol{\beta}, \sigma^2(X^TX)^{-1})$. Since the Gaussian distribution is closed under linear transformations, this means that $\boldsymbol{x}_0^T\hat{\boldsymbol{\beta}} \sim N(\boldsymbol{x}_0^T\boldsymbol{\beta}, \sigma^2\boldsymbol{x}_0^T(X^TX)^{-1}\boldsymbol{x}_0)$, which is univariate. Now, since $E\boldsymbol{x}_0^T\hat{\boldsymbol{\beta}} = \boldsymbol{x}_0^T\boldsymbol{\beta}$, $\boldsymbol{x}_0^T\hat{\boldsymbol{\beta}}$ is an unbiased estimator of $EY_0 = \boldsymbol{x}_0^T\boldsymbol{\beta}$, with distribution as given above. 

## b)

Generally, we know that if $Z \sim N(0,1)$ and $U \sim \chi^2_q$, where $Z$ and $U$ are independent, then $\frac{Z}{\sqrt{U/q}} \sim t_q$. In this case, we can set $Z = \frac{\boldsymbol{x}_0^T\hat{\boldsymbol{\beta}}-\boldsymbol{x}_0^T\boldsymbol{\beta}}{\sqrt{\sigma^2\boldsymbol{x}_0^T(X^TX)^{-1}\boldsymbol{x}_0)}}$ and $U = \frac{1}{\sigma^2}\text{SSE} = \frac{(n-p)\hat{\sigma}^2}{\sigma^2} \sim \chi^2_{n-p}$. Moreover, $Z$ and $U$ are independent, because $\hat{\boldsymbol{\beta}}$ and $\hat{\sigma}^2$ are independent. Hence, the estimator 

$$
  T = \frac{Z}{\sqrt{U/q}} = \frac{\frac{\boldsymbol{x}_0^T\hat{\boldsymbol{\beta}}-\boldsymbol{x}_0^T\boldsymbol{\beta}}{\sqrt{\sigma^2\boldsymbol{x}_0^T(X^TX)^{-1}\boldsymbol{x}_0)}}}{\sqrt{\frac{(n-p)\hat{\sigma}^2}{\sigma^2}/(n-p)}} = \frac{\boldsymbol{x}_0^T\hat{\boldsymbol{\beta}}-\boldsymbol{x}_0^T\boldsymbol{\beta}}{\sqrt{\hat{\sigma}^2\boldsymbol{x}_0^T(X^TX)^{-1}\boldsymbol{x}_0)}} \sim t_{n-p}. 
$$

This means that 

$$
\begin{split}
  &-t \leq \frac{\boldsymbol{x}_0^T\hat{\boldsymbol{\beta}}-\boldsymbol{x}_0^T\boldsymbol{\beta}}{\sqrt{\hat{\sigma}^2\boldsymbol{x}_0^T(X^TX)^{-1}\boldsymbol{x}_0}} \leq t, \\
  &\iff \boldsymbol{x}_0^T\hat{\boldsymbol{\beta}} - t\hat{\sigma}\sqrt{\boldsymbol{x}_0^T(X^TX)^{-1}\boldsymbol{x}_0)} \leq \boldsymbol{x}_0^T\boldsymbol{\beta} \leq \boldsymbol{x}_0^T\hat{\boldsymbol{\beta}} + t\hat{\sigma}\sqrt{\boldsymbol{x}_0^T(X^TX)^{-1}\boldsymbol{x}_0)}, \\
  &\iff \boldsymbol{x}_0^T\hat{\boldsymbol{\beta}} - t\hat{\sigma}\sqrt{\boldsymbol{x}_0^T(X^TX)^{-1}\boldsymbol{x}_0)} \leq EY_0 \leq \boldsymbol{x}_0^T\hat{\boldsymbol{\beta}} + t\hat{\sigma}\sqrt{\boldsymbol{x}_0^T(X^TX)^{-1}\boldsymbol{x}_0)}.
\end{split}
$$

Hence, 

$$
\begin{split}
1-\alpha &= P\left(-t_{\alpha/2} \leq \frac{\boldsymbol{x}_0^T\hat{\boldsymbol{\beta}}-\boldsymbol{x}_0^T\boldsymbol{\beta}}{\sqrt{\hat{\sigma}^2\boldsymbol{x}_0^T(X^TX)^{-1}\boldsymbol{x}_0}} \leq t_{\alpha/2} \right) \\ &= P\left(\boldsymbol{x}_0^T\hat{\boldsymbol{\beta}} - t_{\alpha/2}\hat{\sigma}\sqrt{\boldsymbol{x}_0^T(X^TX)^{-1}\boldsymbol{x}_0} \leq EY_0 \leq \boldsymbol{x}_0^T\hat{\boldsymbol{\beta}} + t_{\alpha/2}\hat{\sigma}\sqrt{\boldsymbol{x}_0^T(X^TX)^{-1}\boldsymbol{x}_0} \right),
\end{split}
$$

which means that $\boldsymbol{x}_0^T\hat{\boldsymbol{\beta}} \pm t_{\alpha/2}\hat{\sigma}\sqrt{\boldsymbol{x}_0^T(X^TX)^{-1}\boldsymbol{x}_0)}$ is a $100(1-\alpha)\%$ confidence interval for $EY_0$. 

## c)

A similar process to the one used in *b)* is used. For a future observation $Y_0$ we can derive that $Y_0 - \boldsymbol{x}_0^T\hat{\boldsymbol{\beta}} \sim N(0, \sigma^2(1 + \boldsymbol{x}_0^T(X^TX)^{-1}\boldsymbol{x}_0))$, since $Y_0 = \boldsymbol{x}_0^T\boldsymbol{\beta} + \varepsilon_0$ and $\boldsymbol{x}_0^T\hat{\boldsymbol{\beta}}$ is an unbiased estimator of $EY_0$. Setting $Z = \frac{Y_0 - \boldsymbol{x}_0^T\hat{\boldsymbol{\beta}}}{\sigma\sqrt{(1 + \boldsymbol{x}_0^T(X^TX)^{-1}\boldsymbol{x}_0)}}$ and set $U$ as in *b)*. Solving the same inequalities as in *b)* then gives

$$
1-\alpha = P\left(\boldsymbol{x}_0^T\hat{\boldsymbol{\beta}} - t_{\alpha/2}\hat{\sigma}\sqrt{1+\boldsymbol{x}_0^T(X^TX)^{-1}\boldsymbol{x}_0} \leq Y_0 \leq \boldsymbol{x}_0^T\hat{\boldsymbol{\beta}} + t_{\alpha/2}\hat{\sigma}\sqrt{1+\boldsymbol{x}_0^T(X^TX)^{-1}\boldsymbol{x}_0} \right),
$$

which means that $\boldsymbol{x}_0^T\hat{\boldsymbol{\beta}} \pm  t_{\alpha/2}\hat{\sigma}\sqrt{1+\boldsymbol{x}_0^T(X^TX)^{-1}\boldsymbol{x}_0}$ is a $100(1-\alpha)\%$ prediction interval for $Y_0$. \textcolor{red}{Why does $Y_0$ independent of $\boldsymbol{\varepsilon}$ give independence from $\boldsymbol{x}_0^T\hat{\boldsymbol{\beta}}$?}

## d)

```{r}
acidrain <-read.table("https://www.math.ntnu.no/emner/TMA4267/2018v/acidrain.txt",header=TRUE)
fit <- lm(y~., data = acidrain)

# Confidence interval: Done manually via the equations found in previous tasks. 
X <- model.matrix(fit)
x0 <- c(1, 3, 50, 1, 50, 2, 1, 0)
n <- dim(X)[1]
p <- dim(X)[2]
quantile <- qt(0.025, n-p,lower.tail = FALSE)
prediction <- t(x0)%*%fit$coefficients
upper.conf <- prediction + quantile*summary(fit)$sigma*sqrt(t(x0)%*%solve(t(X)%*%X)%*%x0)
lower.conf <- prediction - quantile*summary(fit)$sigma*sqrt(t(x0)%*%solve(t(X)%*%X)%*%x0)
prediction
lower.conf
upper.conf

# Confidence interval: Done in R.
newdata <- data.frame(x1=3,x2=50,x3=1,x4=50,x5=2,x6=1,x7=0)
predict(fit, newdata, level=.95, interval="confidence")

# Prediction interval: Done manually via the equations found in previous tasks. 
upper.pred <- prediction + quantile*summary(fit)$sigma*sqrt(1+t(x0)%*%solve(t(X)%*%X)%*%x0)
lower.pred <- prediction - quantile*summary(fit)$sigma*sqrt(1+t(x0)%*%solve(t(X)%*%X)%*%x0)
prediction
lower.pred
upper.pred

# Prediction interval: Done in R.
predict(fit, newdata, level=.95, interval="prediction")
```

## e)

Calculate $\boldsymbol{x}_0^T(X^TX)^{-1}\boldsymbol{x}_0$ with $\boldsymbol{x}_0^T = (1 \hspace{3mm} x_0)$ and 

$$
X^T = 
\begin{pmatrix} 
    1 & 1 & 1 & \dots & \dots & 1\\
    x_1 & x_2 & x_3 & \dots & \dots & x_n
\end{pmatrix}.
$$

This, combined with the rest of the expression for the confidence interval from *b)*, gives the desired expression for simple linear regression. 

# Problem 2 \hspace{3mm} Plant stress

## a)

* t-value for intercept is missing: This is calculated by the test statistic $\hat{\beta}_{\text{intercept}}/\hat{SE}^2 \approx 16.15942/0.04140 \approx$ `r round(16.15942/0.04140, digits = 4)`. This is the test statistic for testing $H_0: \hat{\beta}_{\text{intercept}} = 0$ vs. $H_1: \hat{\beta}_{\text{intercept}} \neq 0$. 

* Std. Error for D:T is missing: This can be calculated from the same test statistic as in the last bullet point, since we know the t-value for D:T. Hence, $\hat{\beta}_{\text{D:T}}/\hat{SE} = t$ gives $\hat{SE} = \hat{\beta}_{\text{D:T}}/t \approx -0.00242/-0.058 \approx$ `r round(0.00242/0.058, digits = 4)`.

* p-value for D:F:T is missing: This can be calculated as $2P(T \geq t) =$ `2*pt(2.198, 24, lower.tail = F)` $\approx$ `r 2*pt(2.198, 24, lower.tail = F)`. 

* Multiple R-squared is missing: This can be calculated as $1 - \frac{\text{SSE}}{\text{SST}}$. $\text{SSE}$ can be calculated from the formula $(n-p)\hat{\sigma}^2 = (32-8)\hat{\sigma}^2 = 24\hat{\sigma}^2 \approx$ `r 24*0.2342^2`, where $\hat{\sigma}$ is found as `Residual Standard Error` in the summary-table. We also know the F-statistic, which is calculated as $\frac{\text{SSR}/(p-1)}{\text{SSE}/(n-p)} = \frac{(\text{SST}-\text{SSE})/(p-1)}{\text{SSE}/(n-p)} = \frac{(\text{SST}-\text{SSE})/(8-1)}{\text{SSE}/(32-8)} = \frac{(\text{SST}-\text{SSE})/7}{\text{SSE}/24} \approx 105.6$, which gives that $\text{SST} \approx$ `r (105.6*24*0.2342^2)*7/24 + 24*0.2342^2`. Finally, this gives $R^2 \approx$ `r 1-(24*0.2342^2)/((105.6*24*0.2342^2)*7/24 + 24*0.2342^2)`. 

## b)

An estimator could be $\hat{\gamma} = 2^{\hat{\beta}_F - \hat{\beta}_D}$. The expected value and variance of this estimator can be calculated using a first order Taylor expansion. Setting $h(x,y) = 2^{x-y}$ and using a Taylor expansion in $x$ and $y$ of first order gives 

$$
\begin{split}
h(\hat{\beta}_F, \hat{\beta}_D) &\approx h(\beta_F, \beta_D) + h_{\hat{\beta}_F}(\beta_F, \beta_D)(\beta_F - \hat{\beta}_F) + h_{\hat{\beta}_D}(\beta_F, \beta_D)(\beta_D - \hat{\beta}_D) \\
&= 2^{\beta_F-\beta_D} + 2^{\beta_F - \beta_D}(\beta_F - \hat{\beta}_F)\text{ln}(2) + 2^{\beta_F - \beta_D}(\beta_D - \hat{\beta}_D)\text{ln}(2), 
\end{split}
$$

since $h_x(x,y) = \frac{\partial}{\partial x}h(x,y) =  \frac{\partial}{\partial x}2^{x-y} = \frac{\partial}{\partial x}\exp{((x-y)\text{ln}(2))} = 2^{x-y}\text{ln}(2)$. This means that $\text{E}(\hat{\gamma}) = \text{E}(2^{\hat{\beta}_F - \hat{\beta}_D}) = \text{E}(h(\hat{\beta}_F, \hat{\beta}_D)) \approx h(\beta_F, \beta_D) = 2^{\beta_F - \beta_D}$, since $\hat{\beta}_F$ and $\hat{\beta}_D$ are unbiased estimators of $\beta_F$ and $\beta_D$. Moreover, $\text{Var}(\hat{\gamma}) = \text{Var}(2^{\hat{\beta}_F - \hat{\beta}_D}) = \text{Var}(h(\hat{\beta}_F, \hat{\beta}_D)) \approx h_{\hat{\beta}_F}(\beta_F, \beta_D)^2\text{Var}(\hat{\beta}_F) + h_{\hat{\beta}_D}(\beta_F, \beta_D)^2\text{Var}(\hat{\beta}_D) = 2^{2(\beta_F - \beta_D)}(\text{ln}(2))^2(\text{Var}(\hat{\beta}_F)-\text{Var}(\hat{\beta}_D))$. 

From Figure 1, we can get the numerical estimates of the moments, given as



# Problem 3 \hspace{3mm} Multiple testing with plant stress

```{r}
pvalues <- scan("https://www.math.ntnu.no/emner/TMA4267/2018v/damagePvalues.txt")
m <- length(pvalues)
```


## a) 

The family-wise error rate (FWER) is the probability of one or more false positive findings $P(V > 0)$, where $V$ is the number of false positive findings among the $m$ tests. The false discovery rate (FDR) gives the expected proportion of false positive results among the $m$ hypotheses tested. A false positive is the same as a type I error, a case where the null hypothesis is rejected despite it being true. In the case of multiple linear regression this means that it is concluded that there is a linear relationship between the predictors and the response, despite the relationship not existing. 

## b)

Control FWER at level $\alpha = 0.05$ with the Bonferroni method. This gives $\alpha_{\text{loc}} = \frac{0.05}{m} =$ `r 0.05/10000`. In this case one would reject `length(pvalues[pvalues<5e-6])` $=$ `r length(pvalues[pvalues<5e-6])` null-hypotheses in the data. Requirements when using Bonferronis method are 
